src/tls/HSL.Receive.fst
@@ -47,6 +47,9 @@ open HSL.Common
 
 type inc_st_t = G.erased (bytes & in_progress_flt_t)
 
+
+/// inc_st is a pointer to erased data
+
 noeq
 type hsl_state = {
   rgn: Mem.rgn;
@@ -71,23 +74,32 @@ let create r =
   let inc_st = B.malloc r (G.hide (Seq.empty, F_none)) 1ul in
   { rgn = r; inc_st = inc_st }
 
+(***** TODO: these errors should move somewhere
+       so that clients can match on them *****)
+
 assume val parsing_error : TLSError.error
 assume val unexpected_flight_error : TLSError.error
 assume val bytes_remain_error : TLSError.error
 
-noextract
+
+/// Main workhorse of parsing messages
+///
+/// Later we partially apply this function to parse
+/// 1.3, 1.2, and CH and SH messages
+
+inline_for_extraction noextract
 let parse_common
   (#a1:Type) (#k1:R.strong_parser_kind)
   (#p1:LP.parser k1 a1)
-  (validator:LP.validator #k1 #a1 p1)
-  (tag_fn:a1 -> HSMType.handshakeType{
+  (validator:LP.validator #k1 #a1 p1)  //a1, p1, etc. are HSM12, HSM13, or HSM
+  (tag_fn:a1 -> HSMType.handshakeType{  //this refinment is basically capturing lemma_valid_handshake13_valid_handshakeType kind of lemmas
     forall (b:R.slice) (pos:UInt32.t) (h:HS.mem).
       LP.valid p1 h b pos ==>
       (LP.valid HSMType.handshakeType_parser h b pos /\
        LP.contents HSMType.handshakeType_parser h b pos ==
        tag_fn (LP.contents p1 h b pos))})
   (#a2:Type) (#k2:R.strong_parser_kind)
-  (#p2:LP.parser k2 a2) (#cl:LP.clens a1 a2)
+  (#p2:LP.parser k2 a2) (#cl:LP.clens a1 a2)  //a2, p2, etc. are specific kind of messages such as EE, Fin, etc.
   (#gacc:LP.gaccessor p1 p2 cl)
   (tag:HSMType.handshakeType{
     forall (m:a1).
@@ -103,19 +115,19 @@ let parse_common
       (match r with
        | E.Error _ -> True
        | E.Correct None -> True
-       | E.Correct (Some (repr, pos)) ->
+       | E.Correct (Some (repr, pos)) ->  //on a successful parse it returns a valid repr with lens condition
          repr.R.start_pos == from /\
          repr.R.end_pos == pos /\
          R.valid repr h1 /\
          cl.LP.clens_cond (R.value repr)))
          
   = fun b from ->
-    
-    let pos = validator b from in
+
+    let pos = validator b from in  //validator gives us the valid postcondition
 
     if pos <= LP.validator_max_length then begin
       let parsed_tag = HSMType.handshakeType_reader b from in
-      if parsed_tag = tag then
+      if parsed_tag = tag then  //and this dynamic check gives us the lens postcondition
         let r = R.mk b from pos p1 in
         E.Correct (Some (r, pos))
       else E.Error unexpected_flight_error
@@ -123,7 +135,11 @@ let parse_common
     else if pos = LP.validator_error_not_enough_data then E.Correct None
     else E.Error parsing_error
 
-let reset_incremental_state (st:hsl_state)
+
+/// Helper function to reset incremental state
+/// Will be used when we have successfully parsed the requested flight
+
+private let reset_incremental_state (st:hsl_state)
   : Stack unit
     (requires fun h -> B.live h st.inc_st)
     (ensures fun h0 _ h1 ->
@@ -133,7 +149,12 @@ let reset_incremental_state (st:hsl_state)
   =  let inc_st = G.hide (Seq.empty, F_none) in
      B.upd st.inc_st 0ul inc_st
 
-let err_or_insufficient_data
+/// Helper function to handle the error case or the insufficient data case
+///
+/// In the first case, it just returns the error as is
+/// In the second case, it saves the incremental state
+
+private let err_or_insufficient_data
   (#a:Type) (#t:Type)
   (parse_result:TLSError.result (option a))
   (in_progress:in_progress_flt_t)
@@ -164,11 +185,18 @@ let err_or_insufficient_data
       B.upd st.inc_st 0ul inc_st;
       E.Correct None
 
+(*** 1.3 flights ***)
+
+
+/// Specialize the parse_common function for Handshake13 messages
+
 inline_for_extraction noextract
 let parse_hsm13 =
   parse_common
     HSM13.handshake13_validator
     HSM13.tag_of_handshake13
+
+/// And then for specific Handshake13 messages
 
 inline_for_extraction noextract
 let parse_hsm13_ee
@@ -212,26 +240,31 @@ let parse_hsm13_nst
       HSMType.New_session_ticket
       HSM13.handshake13_accessor_new_session_ticket
 
+
+/// The flights parsing code is straightforward if..then..else using the parsing functions above
+
 let receive_flight13_ee_c_cv_fin st b from to =
+  let flt = F13_ee_c_cv_fin in
+
   let r = parse_hsm13_ee b from in
   match r with
   | E.Error _ | E.Correct None ->
-    err_or_insufficient_data r F13_ee_c_cv_fin st b from to
+    err_or_insufficient_data r flt st b from to
   | E.Correct (Some (ee_repr, c_begin)) ->
     let r = parse_hsm13_c b c_begin in
     match r with
     | E.Error _ | E.Correct None ->
-      err_or_insufficient_data r F13_ee_c_cv_fin st b from to
+      err_or_insufficient_data r flt st b from to
     | E.Correct (Some (c_repr, cv_begin)) ->
       let r = parse_hsm13_cv b cv_begin in
       match r with
       | E.Error _ | E.Correct None ->
-        err_or_insufficient_data r F13_ee_c_cv_fin st b from to
+        err_or_insufficient_data r flt st b from to
       | E.Correct (Some (cv_repr, fin_begin)) ->
         let r = parse_hsm13_fin b fin_begin in
         match r with
         | E.Error _ | E.Correct None ->
-          err_or_insufficient_data r F13_ee_c_cv_fin st b from to
+          err_or_insufficient_data r flt st b from to
         | E.Correct (Some (fin_repr, pos)) ->
           if pos <> to then E.Error bytes_remain_error
           else begin
@@ -245,30 +278,32 @@ let receive_flight13_ee_c_cv_fin st b from to =
           end
 
 let receive_flight13_ee_cr_c_cv_fin st b from to =
+  let flt = F13_ee_cr_c_cv_fin in
+
   let r = parse_hsm13_ee b from in
   match r with
   | E.Error _ | E.Correct None ->
-    err_or_insufficient_data r F13_ee_cr_c_cv_fin st b from to
+    err_or_insufficient_data r flt st b from to
   | E.Correct (Some (ee_repr, cr_begin)) ->
     let r = parse_hsm13_cr b cr_begin in
     match r with
     | E.Error _ | E.Correct None ->
-      err_or_insufficient_data r F13_ee_cr_c_cv_fin st b from to
+      err_or_insufficient_data r flt st b from to
     | E.Correct (Some (cr_repr, c_begin)) ->
       let r = parse_hsm13_c b c_begin in
       match r with
       | E.Error _ | E.Correct None ->
-        err_or_insufficient_data r F13_ee_cr_c_cv_fin st b from to
+        err_or_insufficient_data r flt st b from to
       | E.Correct (Some (c_repr, cv_begin)) ->
         let r = parse_hsm13_cv b cv_begin in
         match r with
         | E.Error _ | E.Correct None ->
-          err_or_insufficient_data r F13_ee_cr_c_cv_fin st b from to
+          err_or_insufficient_data r flt st b from to
         | E.Correct (Some (cv_repr, fin_begin)) ->
           let r = parse_hsm13_fin b fin_begin in
           match r with
           | E.Error _ | E.Correct None ->
-            err_or_insufficient_data r F13_ee_cr_c_cv_fin st b from to
+            err_or_insufficient_data r flt st b from to
           | E.Correct (Some (fin_repr, pos)) ->
             if pos <> to then E.Error bytes_remain_error
             else begin
@@ -283,15 +318,17 @@ let receive_flight13_ee_cr_c_cv_fin st b from to =
             end
 
 let receive_flight13_ee_fin st b from to =
+  let flt = F13_ee_fin in
+
   let r = parse_hsm13_ee b from in
   match r with
   | E.Error _ | E.Correct None ->
-    err_or_insufficient_data r F13_ee_fin st b from to
+    err_or_insufficient_data r flt st b from to
   | E.Correct (Some (ee_repr, fin_begin)) ->
     let r = parse_hsm13_fin b fin_begin in
     match r with
     | E.Error _ | E.Correct None ->
-      err_or_insufficient_data r F13_ee_fin st b from to
+      err_or_insufficient_data r flt st b from to
     | E.Correct (Some (fin_repr, pos)) ->
       if pos <> to then E.Error bytes_remain_error
       else begin
@@ -303,10 +340,12 @@ let receive_flight13_ee_fin st b from to =
       end
 
 let receive_flight13_fin st b from to =
+  let flt = F13_fin in
+
   let r = parse_hsm13_fin b from in
   match r with
   | E.Error _ | E.Correct None ->
-    err_or_insufficient_data r F13_fin st b from to
+    err_or_insufficient_data r flt st b from to
   | E.Correct (Some (fin_repr, pos)) ->
     if pos <> to then E.Error bytes_remain_error
     else begin
@@ -315,20 +354,22 @@ let receive_flight13_fin st b from to =
     end
 
 let receive_flight13_c_cv_fin st b from to =
+  let flt = F13_c_cv_fin in
+
   let r = parse_hsm13_c b from in
   match r with
   | E.Error _ | E.Correct None ->
-    err_or_insufficient_data r F13_c_cv_fin st b from to
+    err_or_insufficient_data r flt st b from to
   | E.Correct (Some (c_repr, cv_begin)) ->
     let r = parse_hsm13_cv b cv_begin in
     match r with
     | E.Error _ | E.Correct None ->
-      err_or_insufficient_data r F13_c_cv_fin st b from to
+      err_or_insufficient_data r flt st b from to
     | E.Correct (Some (cv_repr, fin_begin)) ->
       let r = parse_hsm13_fin b fin_begin in
       match r with
       | E.Error _ | E.Correct None ->
-        err_or_insufficient_data r F13_c_cv_fin st b from to
+        err_or_insufficient_data r flt st b from to
       | E.Correct (Some (fin_repr, pos)) ->
         if pos <> to then E.Error bytes_remain_error
         else begin
@@ -340,10 +381,12 @@ let receive_flight13_c_cv_fin st b from to =
         end
 
 let receive_flight13_eoed st b from to =
+  let flt = F13_eoed in
+
   let r = parse_hsm13_eoed b from in
   match r with
   | E.Error _ | E.Correct None ->
-    err_or_insufficient_data r F13_eoed st b from to
+    err_or_insufficient_data r flt st b from to
   | E.Correct (Some (eoed_repr, pos)) ->
     if pos <> to then E.Error bytes_remain_error
     else begin
@@ -352,10 +395,12 @@ let receive_flight13_eoed st b from to =
     end
 
 let receive_flight13_nst st b from to =
+  let flt = F13_nst in
+
   let r = parse_hsm13_nst b from in
   match r with
   | E.Error _ | E.Correct None ->
-    err_or_insufficient_data r F13_nst st b from to
+    err_or_insufficient_data r flt st b from to
   | E.Correct (Some (nst_repr, pos)) ->
     if pos <> to then E.Error bytes_remain_error
     else begin
@@ -363,11 +408,20 @@ let receive_flight13_nst st b from to =
       E.Correct (Some ({ nst_msg = nst_repr }))
     end
 
+
+(*** 1.2 flights ***)
+
+
+/// Specialize the parse_common function for Handshake12 messages
+
 inline_for_extraction noextract
 let parse_hsm12 =
   parse_common
     HSM12.handshake12_validator
     HSM12.tag_of_handshake12
+
+
+/// And then for specific Handshake12 messages
 
 inline_for_extraction noextract
 let parse_hsm12_c
@@ -412,20 +466,22 @@ let parse_hsm12_cke
       HSM12.handshake12_accessor_client_key_exchange
 
 let receive_flight12_c_ske_shd st b from to =
+  let flt = F12_c_ske_shd in
+
   let r = parse_hsm12_c b from in
   match r with
   | E.Error _ | E.Correct None ->
-    err_or_insufficient_data r F12_c_ske_shd st b from to
+    err_or_insufficient_data r flt st b from to
   | E.Correct (Some (c_repr, ske_begin)) ->
     let r = parse_hsm12_ske b ske_begin in
     match r with
     | E.Error _ | E.Correct None ->
-      err_or_insufficient_data r F12_c_ske_shd st b from to
+      err_or_insufficient_data r flt st b from to
     | E.Correct (Some (ske_repr, shd_begin)) ->
       let r = parse_hsm12_shd b shd_begin in
       match r with
       | E.Error _ | E.Correct None ->
-        err_or_insufficient_data r F12_c_ske_shd st b from to
+        err_or_insufficient_data r flt st b from to
       | E.Correct (Some (shd_repr, pos)) ->
         if pos <> to then E.Error bytes_remain_error
         else begin
@@ -437,25 +493,27 @@ let receive_flight12_c_ske_shd st b from to =
         end
 
 let receive_flight12_c_ske_cr_shd st b from to =
+  let flt = F12_c_ske_cr_shd in
+
   let r = parse_hsm12_c b from in
   match r with
   | E.Error _ | E.Correct None ->
-    err_or_insufficient_data r F12_c_ske_cr_shd st b from to
+    err_or_insufficient_data r flt st b from to
   | E.Correct (Some (c_repr, ske_begin)) ->
     let r = parse_hsm12_ske b ske_begin in
     match r with
     | E.Error _ | E.Correct None ->
-      err_or_insufficient_data r F12_c_ske_cr_shd st b from to
+      err_or_insufficient_data r flt st b from to
     | E.Correct (Some (ske_repr, cr_begin)) ->
       let r = parse_hsm12_cr b cr_begin in
       match r with
       | E.Error _ | E.Correct None ->
-        err_or_insufficient_data r F12_c_ske_cr_shd st b from to
+        err_or_insufficient_data r flt st b from to
       | E.Correct (Some (cr_repr, shd_begin)) ->
         let r = parse_hsm12_shd b shd_begin in
         match r with
         | E.Error _ | E.Correct None ->
-          err_or_insufficient_data r F12_c_ske_cr_shd st b from to
+          err_or_insufficient_data r flt st b from to
         | E.Correct (Some (shd_repr, pos)) ->
           if pos <> to then E.Error bytes_remain_error
           else begin
@@ -469,10 +527,12 @@ let receive_flight12_c_ske_cr_shd st b from to =
           end
 
 let receive_flight12_fin st b from to =
+  let flt = F12_fin in
+
   let r = parse_hsm12_fin b from in
   match r with
   | E.Error _ | E.Correct None ->
-    err_or_insufficient_data r F12_fin st b from to
+    err_or_insufficient_data r flt st b from to
   | E.Correct (Some (fin_repr, pos)) ->
     if pos <> to then E.Error bytes_remain_error
     else begin
@@ -481,10 +541,12 @@ let receive_flight12_fin st b from to =
     end
 
 let receive_flight12_nst st b from to =
+  let flt = F12_nst in
+
   let r = parse_hsm12_nst b from in
   match r with
   | E.Error _ | E.Correct None ->
-    err_or_insufficient_data r F12_nst st b from to
+    err_or_insufficient_data r flt st b from to
   | E.Correct (Some (nst_repr, pos)) ->
     if pos <> to then E.Error bytes_remain_error
     else begin
@@ -493,10 +555,12 @@ let receive_flight12_nst st b from to =
     end
 
 let receive_flight12_cke st b from to =
+  let flt = F12_cke in
+
   let r = parse_hsm12_cke b from in
   match r with
   | E.Error _ | E.Correct None ->
-    err_or_insufficient_data r F12_cke st b from to
+    err_or_insufficient_data r flt st b from to
   | E.Correct (Some (cke_repr, pos)) ->
     if pos <> to then E.Error bytes_remain_error
     else begin
@@ -504,11 +568,20 @@ let receive_flight12_cke st b from to =
       E.Correct (Some ({ cke_msg = cke_repr }))
     end
 
+
+(*** ClientHello and ServerHello ***)
+
+
+/// Specialize the parse_common function for Handshake messages
+
 inline_for_extraction noextract
 let parse_hsm =
   parse_common
     HSM.handshake_validator
     HSM.tag_of_handshake
+
+
+/// And then for CH and SH
 
 inline_for_extraction noextract
 let parse_hsm_ch
@@ -523,10 +596,12 @@ let parse_hsm_sh
       HSM.handshake_accessor_server_hello
 
 let receive_flight_ch st b from to =
+  let flt = F_ch in
+
   let r = parse_hsm_ch b from in
   match r with
   | E.Error _ | E.Correct None ->
-    err_or_insufficient_data r F_ch st b from to
+    err_or_insufficient_data r flt st b from to
   | E.Correct (Some (ch_repr, pos)) ->
     if pos <> to then E.Error bytes_remain_error
     else begin
@@ -535,10 +610,12 @@ let receive_flight_ch st b from to =
     end
 
 let receive_flight_sh st b from to =
+  let flt = F_sh in
+
   let r = parse_hsm_sh b from in
   match r with
   | E.Error _ | E.Correct None ->
-    err_or_insufficient_data r F_sh st b from to
+    err_or_insufficient_data r flt st b from to
   | E.Correct (Some (sh_repr, pos)) ->
     if pos <> to then E.Error bytes_remain_error
     else begin
